add input generators to Runner and Forker
Runner and Forker now have variants, IRunner and IForker, that
take an input generator module as an argument.

This is an important addition for using the forking lemma in
security games --- reductions usually work with a fixed input
and hence need the basic Forker, but to analyse the probability
of a success event relative to the whole game, we need to average
over different inputs generated by the game and in that case, the
IForker variant becomes useful.

(The diff is quite large, but there's nothing too fancy going on,
it's mostly renaming, changing module and procedure arguments, and
adding the assertions that hops preserve equality of globs of the
input generator I.)

proof/Forking.ec
@@ -87,7 +87,7 @@ module type Forkable = {
   include Stoppable
 }.
 
-module Forker(F : Forkable) = {
+module IForker(I : IGen, F : Forkable) = {
   (* TODO: Might be easier to prove invariants about these if we
    * keep them local? In such case, we would need to return
    * those in run to be able to refer to the results.
@@ -97,9 +97,10 @@ module Forker(F : Forkable) = {
   var r1, r2 : resp_t
 
   (* First run of F, with query and state logging. *)
-  proc fst(i : in_t) : out_t * (log_t list) * (state_t list) = {
+  proc fst() : out_t * (log_t list) * (state_t list) = {
     var sts : state_t list;
     var st : state_t;
+    var i : in_t;
     var o : out_t;
     var q : query_t;
     var r : resp_t;
@@ -108,6 +109,7 @@ module Forker(F : Forkable) = {
     sts <- [];
     Log.log <- [];
 
+    i <@ I.gen();
     q <@ F.init(i);
     c <- 1;
 
@@ -147,7 +149,7 @@ module Forker(F : Forkable) = {
     return (o, Log.log);
   }
 
-  proc run(i : in_t) : int * aux_t * aux_t = {
+  proc run() : int * aux_t * aux_t = {
     var sts : state_t list;
     var st : state_t;
     var o1, o2 : out_t;
@@ -155,7 +157,7 @@ module Forker(F : Forkable) = {
     var a1, a2 : aux_t;
     var q : query_t;
 
-    (o1, log1, sts) <@ fst(i);
+    (o1, log1, sts) <@ fst();
     (j1, a1) <- o1;
     (q, r1) <- nth witness log1 j1;
 
@@ -177,6 +179,49 @@ module Forker(F : Forkable) = {
     return (j, a1, a2);
   }
 }.
+
+(* NOTE: In the pen & paper proof, the authors first show that
+ * the probability bound holds for a forker with a fixed input
+ * and then prove using Jensen's inequality and linearity of
+ * expectation that it also holds when we average over different
+ * inputs.
+ *
+ * Here, we use a slightly different approach. We make the input
+ * generation a part of the forking algorithm and prove the result
+ * in this general setting. The bound for a fixed input is then
+ * obtained for free by using a constant input generator. (This way,
+ * we fully utilize the power of the rew_with_init lemma and do not
+ * have to import other results from the easycrypt-rewinding library
+ * such as reflection.) *)
+
+module Forker(F : Forkable) = {
+  proc run(i : in_t) : int * aux_t * aux_t = {
+    var ret;
+    ConstGen.i <- i;
+    ret <@ IForker(ConstGen, F).run();
+    return ret;
+  }
+}.
+
+module GenThenFork(I : IGen, F : Forkable) = {
+  proc run() : int * aux_t * aux_t = {
+    var i, ret;
+    i <@ I.gen();
+    ret <@ Forker(F).run(i);
+    return ret;
+  }
+}.
+
+equiv gen_then_fork_equiv (I <: IGen {-IForker}) (F <: Forkable {-I, -IForker}) :
+  GenThenFork(I, F).run ~ IForker(I, F).run :
+  ={glob I, glob F} ==> ={glob I, glob F, glob IForker, res}.
+proof.
+proc.
+inline * - Log.
+wp -2 100.
+swap {2} 3 -2.
+sim.
+qed.
 
 section PROOF.
 
@@ -203,6 +248,17 @@ conseq (_ : _ ==> ={glob S, c, q}) => //.
 sim.
 qed.
 
+equiv irunner_log_equiv (I <: IGen {-Log}) (S <: Stoppable {-I, -Log}) :
+  IRunner(I, S, FRO).run ~ IRunner(I, S, Log(FRO)).run :
+  ={glob I, glob S} ==> ={glob I, glob S, res}.
+proof.
+proc.
+rewrite equiv [{2} 2 -(runner_log_equiv S)].
++ sim.
+call (_ : true).
+auto.
+qed.
+
 (* TODO: Log should, at this point, probably be moved outside this file. *)
 hoare run_log_size (S <: Stoppable {-Log}) (O <: Oracle {-Log}) :
   Runner(S, Log(O)).run : Log.log = [] ==> size Log.log = Q.
@@ -225,7 +281,18 @@ auto => />.
 smt(Q_pos).
 qed.
 
-declare module F <: Forkable {-FRO, -Log, -Runner, -Forker}.
+hoare irun_log_size (I <: IGen {-Log}) (S <: Stoppable {-Log}) (O <: Oracle {-Log}) :
+  IRunner(I, S, Log(O)).run : Log.log = [] ==> size Log.log = Q.
+proof.
+proc.
+call (run_log_size S O).
+call (_ : true).
+skip => //.
+qed.
+
+declare module I <: IGen {-Log, -IForker}.
+
+declare module F <: Forkable {-I, -FRO, -Log, -Runner, -IForker}.
 
 (* Coppied from easycrypt-rewinding. *)
 declare axiom F_rewindable :
@@ -268,41 +335,43 @@ qed.
  * successful fork in terms of probabilities of simpler events.
  *)
 
-local lemma fork_pr i &m :
-  Pr[Forker(F).run(i) @ &m : success res.`1] =
-  Pr[Forker(F).run(i) @ &m : Forker.j1 = Forker.j2 /\ success Forker.j1 /\ Forker.r1 <> Forker.r2].
+local lemma fork_pr &m :
+  Pr[IForker(I, F).run() @ &m : success res.`1] =
+  Pr[IForker(I, F).run() @ &m : IForker.j1 = IForker.j2 /\ success IForker.j1 /\ IForker.r1 <> IForker.r2].
 proof.
 byequiv => //.
 proc.
-seq 9 9 : (={glob Forker}).
+seq 9 9 : (={glob IForker}).
 + sim.
 auto => /#.
 qed.
 
-local lemma pr_split i &m :
-  Pr[Forker(F).run(i) @ &m : Forker.j1 = Forker.j2 /\ success Forker.j1 /\ Forker.r1 <> Forker.r2] >=
-  Pr[Forker(F).run(i) @ &m : Forker.j1 = Forker.j2 /\ success Forker.j1] -
-  Pr[Forker(F).run(i) @ &m : success Forker.j1 /\ Forker.r1 = Forker.r2].
+local lemma pr_split &m :
+  Pr[IForker(I, F).run() @ &m : IForker.j1 = IForker.j2 /\ success IForker.j1 /\ IForker.r1 <> IForker.r2] >=
+  Pr[IForker(I, F).run() @ &m : IForker.j1 = IForker.j2 /\ success IForker.j1] -
+  Pr[IForker(I, F).run() @ &m : success IForker.j1 /\ IForker.r1 = IForker.r2].
 proof.
 (* TODO: Cannot use occurence selector with rewrite Pr? *)
 have -> :
-  Pr[Forker(F).run(i) @ &m : Forker.j1 = Forker.j2 /\ success Forker.j1] =
-  Pr[Forker(F).run(i) @ &m : Forker.j1 = Forker.j2 /\ success Forker.j1 /\ Forker.r1 = Forker.r2] +
-  Pr[Forker(F).run(i) @ &m : Forker.j1 = Forker.j2 /\ success Forker.j1 /\ Forker.r1 <> Forker.r2].
-+ by rewrite Pr[mu_split Forker.r1 = Forker.r2]; smt().
+  Pr[IForker(I, F).run() @ &m : IForker.j1 = IForker.j2 /\ success IForker.j1] =
+  Pr[IForker(I, F).run() @ &m : IForker.j1 = IForker.j2 /\ success IForker.j1 /\ IForker.r1 = IForker.r2] +
+  Pr[IForker(I, F).run() @ &m : IForker.j1 = IForker.j2 /\ success IForker.j1 /\ IForker.r1 <> IForker.r2].
++ by rewrite Pr[mu_split IForker.r1 = IForker.r2]; smt().
 have ABC_le_BC :
-  Pr[Forker(F).run(i) @ &m : Forker.j1 = Forker.j2 /\ success Forker.j1 /\ Forker.r1 = Forker.r2] <=
-  Pr[Forker(F).run(i) @ &m : success Forker.j1 /\ Forker.r1 = Forker.r2].
+  Pr[IForker(I, F).run() @ &m : IForker.j1 = IForker.j2 /\ success IForker.j1 /\ IForker.r1 = IForker.r2] <=
+  Pr[IForker(I, F).run() @ &m : success IForker.j1 /\ IForker.r1 = IForker.r2].
 + by rewrite Pr[mu_sub].
 smt().
 qed.
 
 local equiv fst_run_log_equiv log0 :
-  Forker(F).fst ~ Runner(F, Log(FRO)).run :
-  ={arg, glob F} /\ Log.log{2} = log0 ==>
-  ={glob F} /\ res{1}.`1 = res{2} /\ log0 ++ res{1}.`2 = Log.log{2}.
+  IForker(I, F).fst ~ IRunner(I, F, Log(FRO)).run :
+  ={glob I, glob F} /\ Log.log{2} = log0 ==>
+  ={glob I, glob F} /\ res{1}.`1 = res{2} /\ log0 ++ res{1}.`2 = Log.log{2}.
 proof.
 proc => /=.
+inline Runner.
+wp.
 call (_ : true).
 have log_equiv : equiv[
   Log(FRO).get ~ Log(FRO).get :
@@ -322,64 +391,63 @@ while (={q, c, glob F} /\ log0 ++ Log.log{1} = Log.log{2}).
   wp.
   ecall {1} (get_st_preserves_glob (glob F){1}).
   auto => />.
-wp.
-call (_ : true).
+do 2! (wp; call (_ : true)).
 auto => />.
 smt(cats0).
 qed.
 
 local equiv fst_run_equiv :
-  Forker(F).fst ~ Runner(F, FRO).run :
-  ={arg, glob F} ==> ={glob F} /\ res{1}.`1 = res{2}.
+  IForker(I, F).fst ~ IRunner(I, F, FRO).run :
+  ={glob I, glob F} ==> ={glob I, glob F} /\ res{1}.`1 = res{2}.
 proof.
 proc *.
-rewrite equiv [{2} 1 (runner_log_equiv F)].
+rewrite equiv [{2} 1 (irunner_log_equiv I F)].
 exlim (Log.log{2}) => log0.
 call (fst_run_log_equiv log0).
 auto.
 qed.
 
 local hoare fst_log_size :
-  Forker(F).fst : true ==> size res.`2 = Q.
+  IForker(I, F).fst : true ==> size res.`2 = Q.
 proof.
-conseq (fst_run_log_equiv []) (run_log_size F FRO) => /#.
+conseq (fst_run_log_equiv []) (irun_log_size I F FRO) => /#.
 qed.
 
 const pr_collision = 1%r / (size (to_seq (support dresp)))%r.
 
 (* TODO: Decompose? *)
-local lemma pr_succ_resp_eq &m i :
-  Pr[Forker(F).run(i) @ &m : success Forker.j1 /\ Forker.r1 = Forker.r2] <=
-  Pr[Runner(F, FRO).run(i) @ &m : success res.`1] * pr_collision.
+local lemma pr_succ_resp_eq &m :
+  Pr[IForker(I, F).run() @ &m : success IForker.j1 /\ IForker.r1 = IForker.r2] <=
+  Pr[IRunner(I, F, FRO).run() @ &m : success res.`1] * pr_collision.
 proof.
-byphoare (: arg = i /\ glob F = (glob F){m} ==> _) => //.
+byphoare (: glob I = (glob I){m} /\ glob F = (glob F){m} ==> _) => //.
 proc.
-seq 3 : (success Forker.j1)
-  Pr[Runner(F, FRO).run(i) @ &m : success res.`1] pr_collision
+seq 3 : (success IForker.j1)
+  Pr[IRunner(I, F, FRO).run() @ &m : success res.`1] pr_collision
   _ 0%r
-  (size Forker.log1 = Q);
+  (size IForker.log1 = Q);
 last by trivial.
 
-(* #pre ==> size Forker.log1 = Q *)
+(* #pre ==> size IForker.log1 = Q *)
 + wp.
   call fst_log_size.
   auto.
 
-(* #pre ==> success Forker.j1 *)
+(* #pre ==> success IForker.j1 *)
 + wp.
-  call (_ : glob F = (glob F){m} /\ arg = i ==> success res.`1.`1).
+  call (_ : glob I = (glob I){m} /\ glob F = (glob F){m} ==> success res.`1.`1).
   + bypr => &m0 glob_eq.
     byequiv => //.
     conseq fst_run_equiv; smt().
   auto.
 
-(* success Forker.j1 ==> #post *)
+(* success IForker.j1 ==> #post *)
 + inline.
   wp.
-  conseq (_ : _ ==> success Forker.j1 /\ Forker.r1 = (head witness Log.log).`2).
+  conseq (_ : _ ==> success IForker.j1 /\ IForker.r1 = (head witness Log.log).`2).
   + smt(nth_cat size_takel nth0_head).
   (* FIXME: This is rather painful. Call doesn't work in pHL? *)
-  seq 12 : (success Forker.j1 /\ Forker.r1 = (head witness Log.log).`2)
+  seq 12 : (success IForker.j1 /\ IForker.r1 = (head witness Log.log).`2)
     pr_collision 1%r
     _ 0%r;
   1,3,5: trivial; first last.
@@ -391,8 +459,8 @@ last by trivial.
     have -> : (fun r => r0 = r) = pred1 r0 by smt().
     rewrite (mu1_uni_ll _ _ dresp_uni dresp_ll).
     smt(invr_ge0 size_ge0).
-  case (Forker.j1 = Q - 1).
-  (* case: Forker.j1 = Q*)
+  case (IForker.j1 = Q - 1).
+  (* case: IForker.j1 = Q*)
   + rcondf 6.
     + wp; call (_ : true); auto.
     rnd; wp => /=.
@@ -400,10 +468,10 @@ last by trivial.
     move => &hr [[_ succ] _].
     rewrite succ /=.
     apply mu_dresp_eq.
-  (* case: Forker.j1 <> Q *)
+  (* case: IForker.j1 <> Q *)
   unroll 6; rcondt 6.
   + wp; call (_ : true); wp; skip => /#.
-  seq 11 : (success Forker.j1 /\ Forker.r1 = (head witness Log.log).`2)
+  seq 11 : (success IForker.j1 /\ IForker.r1 = (head witness Log.log).`2)
     pr_collision 1%r
     _ 0%r
     (Log.log <> []);
@@ -415,13 +483,13 @@ last by trivial.
     apply mu_dresp_eq.
   hoare.
   rnd; wp.
-  while (Log.log <> [] /\ ! (success Forker.j1 /\ Forker.r1 = (head witness Log.log).`2)).
+  while (Log.log <> [] /\ ! (success IForker.j1 /\ IForker.r1 = (head witness Log.log).`2)).
   + wp; call (_ : true); wp; rnd; wp; skip => /#.
   wp; call (_ : true); skip => /#.
 
-(* ! success Forker.j1 ==> #post *)
+(* ! success IForker.j1 ==> #post *)
 hoare.
-conseq (_ : _ ==> ! success Forker.j1); 1: smt().
+conseq (_ : _ ==> ! success IForker.j1); 1: smt().
 wp.
 call (_ : true) => //.
 call (_ : true).
@@ -431,15 +499,15 @@ qed.
 (* FIXME: The following two lemmas are almost identical.
  * Try to extract the common bits into a separate lemma or
  * reuse the existing PrIntervalToSum (easycrypt-zk) theory. *)
-local lemma pr_split_sum &m i :
-  Pr[Forker(F).run(i) @ &m : Forker.j1 = Forker.j2 /\ success Forker.j1] =
-  bigi predT (fun j => Pr[Forker(F).run(i) @ &m : Forker.j1 = j /\ Forker.j2 = j]) 0 Q.
+local lemma pr_split_sum &m :
+  Pr[IForker(I, F).run() @ &m : IForker.j1 = IForker.j2 /\ success IForker.j1] =
+  bigi predT (fun j => Pr[IForker(I, F).run() @ &m : IForker.j1 = j /\ IForker.j2 = j]) 0 Q.
 proof.
 rewrite /success.
 have -> :
   forall n, 0 <= n =>
-  Pr[Forker(F).run(i) @ &m : Forker.j1 = Forker.j2 /\ 0 <= Forker.j1 && Forker.j1 < n] =
-  bigi predT (fun j => Pr[Forker(F).run(i) @ &m : Forker.j1 = j /\ Forker.j2 = j]) 0 n;
+  Pr[IForker(I, F).run() @ &m : IForker.j1 = IForker.j2 /\ 0 <= IForker.j1 && IForker.j1 < n] =
+  bigi predT (fun j => Pr[IForker(I, F).run() @ &m : IForker.j1 = j /\ IForker.j2 = j]) 0 n;
 [idtac | smt(Q_pos) | trivial].
 apply ge0ind => /=.
 + smt().
@@ -448,21 +516,21 @@ apply ge0ind => /=.
   by rewrite Pr[mu_false].
 move => n n_ge0 ind _.
 rewrite big_int_recr //=.
-rewrite Pr[mu_split Forker.j1 < n].
+rewrite Pr[mu_split IForker.j1 < n].
 have -> : forall b x, ((b /\ 0 <= x < n + 1) /\ x < n) <=> (b /\ 0 <= x < n) by smt().
 rewrite ind //.
 have -> // : forall j1 j2, ((j1 = j2 /\ 0 <= j1 < n + 1) /\ ! j1 < n) <=> (j1 = n /\ j2 = n) by smt().
 qed.
 
-local lemma pr_succ_sum &m i:
-  Pr[Runner(F, FRO).run(i) @ &m : success res.`1] =
-  bigi predT (fun j => Pr[Runner(F, FRO).run(i) @ &m : res.`1 = j]) 0 Q.
+local lemma pr_succ_sum &m :
+  Pr[IRunner(I, F, FRO).run() @ &m : success res.`1] =
+  bigi predT (fun j => Pr[IRunner(I, F, FRO).run() @ &m : res.`1 = j]) 0 Q.
 proof.
 rewrite /success.
 have -> :
   forall n, 0 <= n =>
-  Pr[Runner(F, FRO).run(i) @ &m : 0 <= res.`1 < n] =
-  bigi predT (fun j => Pr[Runner(F, FRO).run(i) @ &m : res.`1 = j]) 0 n;
+  Pr[IRunner(I, F, FRO).run() @ &m : 0 <= res.`1 < n] =
+  bigi predT (fun j => Pr[IRunner(I, F, FRO).run() @ &m : res.`1 = j]) 0 n;
 [idtac | smt(Q_pos) | trivial].
 apply ge0ind => /=.
 + smt().
@@ -479,9 +547,9 @@ qed.
 
 (* STEP 2:
  * At this point, we can focus on the following probability:
- * Pr[Forker(F).run(i) @ &m : Forker.j1 = j /\ Forker.j2 = j].
+ * Pr[IForker(F).run(i) @ &m : IForker.j1 = j /\ IForker.j2 = j].
  *
- * The key observation is that we can replace Forker by a module,
+ * The key observation is that we can replace IForker by a module,
  * that always forks after the j-th query and the probability
  * does not change.
  *
@@ -489,13 +557,14 @@ qed.
  * the module into the shape required by the rew_with_init lemma.
  *)
 
-local module SplitForker(F : Forkable) = {
+local module SplitForker(I : IGen, F : Forkable) = {
   var bad : bool
 
-  (* Forker.fst that runs F only until the first C queries. *)
-  proc fst_partial(i : in_t, C : int) : query_t * (log_t list) * (state_t list) = {
+  (* IForker.fst that runs F only until the first C queries. *)
+  proc fst_partial(C : int) : query_t * (log_t list) * (state_t list) = {
     var sts : state_t list;
     var st : state_t;
+    var i : in_t;
     var o : out_t;
     var q : query_t;
     var r : resp_t;
@@ -504,6 +573,7 @@ local module SplitForker(F : Forkable) = {
     sts <- [];
     Log.log <- [];
 
+    i <@ I.gen();
     q <@ F.init(i);
     c <- 1;
 
@@ -521,8 +591,8 @@ local module SplitForker(F : Forkable) = {
     return (q, Log.log, sts);
   }
 
-  (* Same as Forker.snd, but with state recording. *)
-  (* TODO: Consider adding state recording to Forker.snd. *)
+  (* Same as IForker.snd, but with state recording. *)
+  (* TODO: Consider adding state recording to IForker.snd. *)
   proc snd(q : query_t, c : int) : out_t * (log_t list) * (state_t list) = {
     var sts : state_t list;
     var st : state_t;
@@ -548,13 +618,13 @@ local module SplitForker(F : Forkable) = {
     return (o, Log.log, sts);
   }
 
-  proc fst(i : in_t, C : int) : out_t * (log_t list) * (state_t list) = {
+  proc fst(C : int) : out_t * (log_t list) * (state_t list) = {
     var sts, sts1, sts2 : state_t list;
     var log, log1, log2 : log_t list;
     var q : query_t;
     var o : out_t;
 
-    (q, log1, sts1) <@ fst_partial(i, C);
+    (q, log1, sts1) <@ fst_partial(C);
     (o, log2, sts2) <@ snd(q, C);
     sts <- sts1 ++ sts2;
     log <- log1 ++ log2;
@@ -562,9 +632,9 @@ local module SplitForker(F : Forkable) = {
     return (o, log, sts);
   }
 
-  (* Forker.run with bad event logging, with some unnecessary bits removed
+  (* IForker.run with bad event logging, with some unnecessary bits removed
    * (e.g., we don't care about aux output nor the two responses to q) *)
-  proc run1(i : in_t, j : int) : int * int * aux_t * aux_t * (log_t list) * (log_t list) = {
+  proc run1(j : int) : int * int * aux_t * aux_t * (log_t list) * (log_t list) = {
     var sts1, _sts2 : state_t list;
     var st : state_t;
     var log1, log2 : log_t list;
@@ -573,7 +643,7 @@ local module SplitForker(F : Forkable) = {
     var a1, a2 : aux_t;
     var q : query_t;
 
-    (o1, log1, sts1) <@ fst(i, j + 1);
+    (o1, log1, sts1) <@ fst(j + 1);
     (j1, a1) <- o1;
 
     bad <- false;
@@ -594,7 +664,7 @@ local module SplitForker(F : Forkable) = {
   }
 
   (* Same as run1, except we always rewind to the j-th query. *)
-  proc run2(i : in_t, j : int) : int * int * aux_t * aux_t * (log_t list) * (log_t list) = {
+  proc run2(j : int) : int * int * aux_t * aux_t * (log_t list) * (log_t list) = {
     var sts1, _sts2 : state_t list;
     var st : state_t;
     var log1, log2 : log_t list;
@@ -603,7 +673,7 @@ local module SplitForker(F : Forkable) = {
     var a1, a2 : aux_t;
     var q : query_t;
 
-    (o1, log1, sts1) <@ fst(i, j + 1);
+    (o1, log1, sts1) <@ fst(j + 1);
     (j1, a1) <- o1;
 
     bad <- false;
@@ -629,36 +699,37 @@ local module SplitForker(F : Forkable) = {
 local lemma fst_split_equiv C :
   1 <= C <= Q =>
   equiv[
-    Forker(F).fst ~ SplitForker(F).fst :
-    ={glob F} /\ arg{1} = arg{2}.`1 /\ arg{2}.`2 = C ==> ={glob F, res}
+    IForker(I, F).fst ~ SplitForker(I, F).fst :
+    ={glob I, glob F} /\ arg{2} = C ==> ={glob I, glob F, res}
   ].
 proof.
 move => C_range.
 proc.
-inline SplitForker(F).fst_partial SplitForker(F).snd Log.
+inline SplitForker(I, F).fst_partial SplitForker(I, F).snd Log.
 wp.
 call (_ : true).
 wp.
 call (_ : true); 1: auto.
 wp.
 call (_ : true).
-splitwhile{1} 5 : c < C.
-conseq (_ : _ ==> ={glob F} /\ q{1} = q1{2} /\ Log.log{1} = log1{2} ++ Log.log{2} /\ sts{1} = sts1{2} ++ sts3{2}) => />.
+splitwhile{1} 6 : c < C.
+conseq (_ : _ ==> ={glob I, glob F} /\ q{1} = q1{2} /\ Log.log{1} = log1{2} ++ Log.log{2} /\ sts{1} = sts1{2} ++ sts3{2}) => />.
 + smt(catA).
-while (={glob F} /\ q{1} = q1{2} /\ Log.log{1} = log1{2} ++ Log.log{2} /\ sts{1} = sts1{2} ++ sts3{2} /\ c{1} = c0{2}).
+while (={glob I, glob F} /\ q{1} = q1{2} /\ Log.log{1} = log1{2} ++ Log.log{2} /\ sts{1} = sts1{2} ++ sts3{2} /\ c{1} = c0{2}).
 + wp. call (_ : true). wp. call (_ : true). auto. wp. call (_ : true). skip => />. smt(catA).
 wp.
-conseq (_ : _ ==> ={glob F} /\ q{1} = q0{2} /\ Log.log{1} = Log.log{2} /\ sts{1} = sts0{2} /\ c{1} = C) => />.
+conseq (_ : _ ==> ={glob I, glob F} /\ q{1} = q0{2} /\ Log.log{1} = Log.log{2} /\ sts{1} = sts0{2} /\ c{1} = C) => />.
 + smt(cats0).
-while (={glob F} /\ q{1} = q0{2} /\ Log.log{1} = Log.log{2} /\ sts{1} = sts0{2} /\ c{1} = c{2} /\ c{1} <= C /\ C0{2} = C).
+while (={glob I, glob F} /\ q{1} = q0{2} /\ Log.log{1} = Log.log{2} /\ sts{1} = sts0{2} /\ c{1} = c{2} /\ c{1} <= C /\ C0{2} = C).
 + wp. call (_ : true). wp. call (_ : true). auto. wp. call (_ : true). skip => />. smt().
 wp.
+call (_ : true).
 call (_ : true).
 auto => /#.
 qed.
 
 local equiv snd_equiv :
-  Forker(F).snd ~ SplitForker(F).snd :
+  IForker(I, F).snd ~ SplitForker(I, F).snd :
   ={glob F, arg} ==> ={glob F} /\ res{1}.`1 = res{2}.`1 /\ res{1}.`2 = res{2}.`2.
 proof.
 proc => /=.
@@ -674,11 +745,11 @@ qed.
 local lemma run_run1_equiv j :
   0 <= j < Q =>
   equiv[
-    Forker(F).run ~ SplitForker(F).run1 :
-    ={glob F} /\ (arg{1}, j) = arg{2} ==>
-    ={glob F} /\ Forker.j1{1} = res{2}.`1 /\ Forker.j2{1} = res{2}.`2 /\
+    IForker(I, F).run ~ SplitForker(I, F).run1 :
+    ={glob I, glob F} /\ arg{2} = j ==>
+    ={glob I, glob F} /\ IForker.j1{1} = res{2}.`1 /\ IForker.j2{1} = res{2}.`2 /\
       res{1}.`2 = res{2}.`3 /\ res{1}.`3 = res{2}.`4 /\
-      Forker.log1{1} = res{2}.`5 /\ Forker.log2{1} = res{2}.`6
+      IForker.log1{1} = res{2}.`5 /\ IForker.log2{1} = res{2}.`6
   ].
 proof.
 move => j_range.
@@ -691,10 +762,10 @@ call (fst_split_equiv (j + 1)); 1: smt().
 auto => /#.
 qed.
 
-local lemma pr_run1_eq &m i j :
+local lemma pr_run1_eq &m j :
   0 <= j < Q =>
-  Pr[Forker(F).run(i) @ &m : Forker.j1 = j /\ Forker.j2 = j] =
-  Pr[SplitForker(F).run1(i, j) @ &m : res.`1 = j /\ res.`2 = j].
+  Pr[IForker(I, F).run() @ &m : IForker.j1 = j /\ IForker.j2 = j] =
+  Pr[SplitForker(I, F).run1(j) @ &m : res.`1 = j /\ res.`2 = j].
 proof.
 move => j_range.
 byequiv => //.
@@ -703,30 +774,37 @@ qed.
 
 (* TODO: Try to prove this using pRHL, i.e., without using
  * the syntactic byupto tactic. *)
-local lemma pr_run2_ineq &m i j :
-  Pr[SplitForker(F).run1(i, j) @ &m : res.`1 = j /\ res.`2 = j] >=
-  Pr[SplitForker(F).run2(i, j) @ &m : res.`1 = j /\ res.`2 = j].
+local lemma pr_run2_ineq &m j :
+  Pr[SplitForker(I, F).run1(j) @ &m : res.`1 = j /\ res.`2 = j] >=
+  Pr[SplitForker(I, F).run2(j) @ &m : res.`1 = j /\ res.`2 = j].
 proof.
 have :
-  Pr[SplitForker(F).run2(i, j) @ &m : res.`1 = j /\ res.`2 = j] <=
-    Pr[SplitForker(F).run1(i, j) @ &m : res.`1 = j /\ res.`2 = j] +
-  Pr[SplitForker(F).run2(i, j) @ &m : (res.`1 = j /\ res.`2 = j) /\ SplitForker.bad].
+  Pr[SplitForker(I, F).run2(j) @ &m : res.`1 = j /\ res.`2 = j] <=
+    Pr[SplitForker(I, F).run1(j) @ &m : res.`1 = j /\ res.`2 = j] +
+  Pr[SplitForker(I, F).run2(j) @ &m : (res.`1 = j /\ res.`2 = j) /\ SplitForker.bad].
 + byupto.
 have -> :
-  Pr[SplitForker(F).run2(i, j) @ &m : (res.`1 = j /\ res.`2 = j) /\ SplitForker.bad] = 0%r.
-+ byphoare (_ : arg.`2 = j ==> _) => //.
+  Pr[SplitForker(I, F).run2(j) @ &m : (res.`1 = j /\ res.`2 = j) /\ SplitForker.bad] = 0%r.
++ byphoare (_ : arg = j ==> _) => //.
   hoare.
   proc => /=.
   conseq (_ : _ ==> !(j1 = j /\ SplitForker.bad)); 1: smt().
-  wp; do 3! (call (_ : true) => //; wp).
+  do 3! (wp; call (_ : true) => //).
 trivial.
 qed.
 
 (* Need to transform SplitForker.run2 into a form
  * that is suitable for application of the rew_with_init lemma. *)
 
-local module RewindWrapper(F : Forkable) = {
+local module InitWrapper(I : IGen, F : Forkable) = {
+  proc init(j : int) : query_t * int * (log_t list) = {
+    var q, log, sts;
+    (q, log, sts) <@ SplitForker(I, F).fst_partial(j + 1);
+    return (q, j, log);
+  }
+}.
 
+local module RewindWrapper(I : IGen, F : Forkable) = {
   (* FIXME: Need to handle bad var in SplitForker and
    * show that this module is rewindable. *)
   proc getState() : state_t = {
@@ -739,17 +817,10 @@ local module RewindWrapper(F : Forkable) = {
     F.setState(st);
   }
 
-  proc init(ij : in_t * int) : query_t * int * (log_t list) = {
-    var i, j, q, log, sts;
-    (i, j) <- ij;
-    (q, log, sts) <@ SplitForker(F).fst_partial(i, j + 1);
-    return (q, j, log);
-  }
-
   proc run(q_j_log : query_t * int * (log_t list)) : out_t * (log_t list) = {
     var q, o, log, log', sts, j;
     (q, j, log) <- q_j_log;
-    (o, log', sts) <@ SplitForker(F).snd(q, j + 1);
+    (o, log', sts) <@ SplitForker(I, F).snd(q, j + 1);
     log <- log ++ log';
     return (o, log);
   }
@@ -757,10 +828,10 @@ local module RewindWrapper(F : Forkable) = {
 
 (* This matches the QQ module in easycrypt-rewinding. *)
 (* FIXME: Clone and instantiate RewWithInit.. *)
-local type iat = in_t * int.
-local module InitRewinder(F : Forkable) = {
-  module A = RewindWrapper(F)
-  module B = RewindWrapper(F)
+local type iat = int.
+local module InitRewinder(I : IGen, F : Forkable) = {
+  module A = RewindWrapper(I, F)
+  module B = InitWrapper(I, F)
 
   proc main(i:iat) = {
     var s, r0, r1, r2;
@@ -781,98 +852,99 @@ local module InitRewinder(F : Forkable) = {
 }.
 
 local equiv rewinder_run_equiv :
-  InitRewinder(F).main_run ~ SplitForker(F).fst :
-  ={glob F} /\ arg{1}.`1 = arg{2}.`1 /\ arg{1}.`2 + 1 = arg{2}.`2  ==>
-  ={glob F} /\ res{1}.`2 = (res{2}.`1, res{2}.`2).
+  InitRewinder(I, F).main_run ~ SplitForker(I, F).fst :
+  ={glob I, glob F} /\ arg{1} + 1 = arg{2}  ==>
+  ={glob I, glob F} /\ res{1}.`2 = (res{2}.`1, res{2}.`2).
 proof.
 proc => /=.
 inline InitRewinder.
 wp.
 call (_ : ={glob F}); 1: sim.
 wp.
-call (_ : ={glob F}); 1: sim.
+call (_ : ={glob I, glob F}); 1: sim.
 auto => />.
 qed.
 
 local lemma main_run_equiv j log0 :
   0 <= j < Q =>
   equiv[
-    Runner(F, Log(FRO)).run ~ InitRewinder(F).main_run :
-    ={glob F} /\ (arg{1}, j) = arg{2} /\ Log.log{1} = log0 ==>
-    res{1} = res{2}.`2.`1 /\ Log.log{1} = log0 ++ res{2}.`2.`2
+    IRunner(I, F, Log(FRO)).run ~ InitRewinder(I, F).main_run :
+    ={glob I, glob F} /\ arg{2} = j /\ Log.log{1} = log0 ==>
+    ={glob I} /\ res{1} = res{2}.`2.`1 /\ Log.log{1} = log0 ++ res{2}.`2.`2
   ].
 proof.
 move => j_range.
 transitivity
-  Forker(F).fst
-  (={glob F, arg} /\ Log.log{1} = log0 ==> res{1} = res{2}.`1 /\ Log.log{1} = log0 ++ res{2}.`2)
-  (={glob F} /\ (arg{1}, j) = arg{2} ==> res{1}.`1 = res{2}.`2.`1 /\ res{1}.`2 = res{2}.`2.`2);
+  IForker(I, F).fst
+  (={glob I, glob F} /\ Log.log{1} = log0 ==> ={glob I} /\ res{1} = res{2}.`1 /\ Log.log{1} = log0 ++ res{2}.`2)
+  (={glob I, glob F} /\ arg{2} = j ==> ={glob I} /\ res{1}.`1 = res{2}.`2.`1 /\ res{1}.`2 = res{2}.`2.`2);
 1,2: smt().
 + by symmetry; conseq (fst_run_log_equiv log0).
 transitivity
-  SplitForker(F).fst
-  (={glob F} /\ (arg{1}, j + 1) = arg{2} ==> ={res})
-  (={glob F} /\ arg{1}.`1 = arg{2}.`1 /\ arg{1}.`2 = arg{2}.`2 + 1 ==> res{1}.`1 = res{2}.`2.`1 /\ res{1}.`2 = res{2}.`2.`2).
+  SplitForker(I, F).fst
+  (={glob I, glob F} /\ arg{2} = j + 1 ==> ={glob I, res})
+  (={glob I, glob F} /\ arg{1} = arg{2} + 1 ==> ={glob I} /\ res{1}.`1 = res{2}.`2.`1 /\ res{1}.`2 = res{2}.`2.`2).
 + move => &1 &2 rel.
-  exists (glob F){1} (arg{1}, j + 1) => /#.
+  exists (glob F){1} (glob I){1} (j + 1) => /#.
 + smt().
 + conseq (fst_split_equiv (j + 1) _) => /#.
 symmetry; conseq rewinder_run_equiv => /#.
 qed.
 
-local lemma pr_wrapper_run &m i j :
+local lemma pr_wrapper_run &m j :
   0 <= j < Q =>
-  Pr[Runner(F, FRO).run(i) @ &m : res.`1 = j] =
-  Pr[InitRewinder(F).main_run((i, j)) @ &m : res.`2.`1.`1 = j].
+  Pr[IRunner(I, F, FRO).run() @ &m : res.`1 = j] =
+  Pr[InitRewinder(I, F).main_run(j) @ &m : res.`2.`1.`1 = j].
 proof.
 move => j_range.
 byequiv => //.
 proc *.
-rewrite equiv [{1} 1 (runner_log_equiv F)].
+rewrite equiv [{1} 1 (irunner_log_equiv I F)].
 exlim (Log.log{1}) => log0.
 call (main_run_equiv j log0).
 auto.
 qed.
 
+(* TODO: This proof really needs some refactoring... *)
 local lemma init_rew_split_equiv j :
   0 <= j < Q =>
   equiv[
-    SplitForker(F).run2 ~ InitRewinder(F).main :
-    ={glob F, arg} /\ arg{1}.`2 = j ==>
+    SplitForker(I, F).run2 ~ InitRewinder(I, F).main :
+    ={glob I, glob F, arg} /\ arg{1} = j ==>
     (* FIXME: Consider changing the return type of SplitForker.run2 *)
     let (j1, j2, a1, a2, log1, log2) = res{1} in
-    ((j1, a1), log1) = res{2}.`1.`2 /\ ((j2, a2), log2) = res{2}.`2.`2
+    ={glob I} /\ ((j1, a1), log1) = res{2}.`1.`2 /\ ((j2, a2), log2) = res{2}.`2.`2
   ].
 proof.
 move => j_range.
 proc => /=.
-inline InitRewinder SplitForker(F).fst.
+inline InitRewinder SplitForker(I, F).fst.
 wp.
 call (_ : ={glob F}); 1: sim.
 wp.
 call (_ : true).
 wp => /=.
 conseq (_ : _ ==>
-  ={glob F, o} /\
+  ={glob I, glob F, o} /\
   nth witness (sts10{1} ++ sts2{1}) j = s{2} /\
   ((nth witness (log10{1} ++ log20{1}) j).`1, j, take j (log10{1} ++ log20{1})) = r0{2} /\
   log10{1} = log0{2} /\ log20{1} = log'{2}
 ); 1: smt().
-seq 3 4 : (={glob F} /\ C{1} = j + 1 /\ (q0{1}, j, log10{1}) = r0{2} /\
+seq 2 3 : (={glob I, glob F} /\ C{1} = j + 1 /\ (q0{1}, j, log10{1}) = r0{2} /\
   size log10{1} = j /\ size sts10{1} = j).
 + wp.
-  call (_ : ={glob F, arg} /\ arg{1}.`2 = j + 1 ==> ={glob F, res} /\ size res{1}.`2 = j /\ size res{1}.`3 = j).
+  call (_ : ={glob I, glob F, arg} /\ arg{1} = j + 1 ==> ={glob I, glob F, res} /\ size res{1}.`2 = j /\ size res{1}.`3 = j).
   + proc.
-    while (={glob F, q, Log.log, sts, c, C} /\ c{1} <= C{1} /\ size Log.log{1} + 1 = c{1} /\ size sts{1} + 1 = c{1}).
+    while (={glob I, glob F, q, Log.log, sts, c, C} /\ c{1} <= C{1} /\ size Log.log{1} + 1 = c{1} /\ size sts{1} + 1 = c{1}).
     + wp. call (_ : true). inline. wp. rnd. wp. call (_ : true). skip => />. smt(size_cat).
-    wp. call (_ : true). wp. skip => /#.
+    wp. call (_ : true). wp. call (_ : true). wp. skip => /#.
   wp. skip => />.
 
 (* TODO: Try to redefine the Forkers/Runner so that there is no oracle
  * call after the while loop. This way we could perhaps avoid some of
  * the case analysis? *)
-inline SplitForker(F).snd Log.
-conseq (_ : _ ==> ={glob F, o} /\
+inline SplitForker(I, F).snd Log.
+conseq (_ : _ ==> ={glob I, glob F, o} /\
   head witness sts2{1} = s{2} /\
   ((head witness log20{1}).`1, j, log10{1}) = r0{2} /\
   log10{1} = log0{2} /\ log20{1} = log'{2}
@@ -904,7 +976,7 @@ rcondt {2} 3.
 + move => &n. wp. call (_ : true). skip. smt().
 call (_ : true).
 while (
-  ={glob F, c, Log.log} /\ q1{1} = q2{2} /\
+  ={glob I, glob F, c, Log.log} /\ q1{1} = q2{2} /\
   head witness sts0{1} = s{2} /\ sts0{1} <> [] /\
   ((head witness Log.log{1}).`1, j, log0{2}) = r0{2} /\ Log.log{1} <> []
 ).
@@ -917,23 +989,23 @@ skip => />.
 smt(head_cons).
 qed.
 
-local lemma pr_wrapper_main &m i j :
+local lemma pr_wrapper_main &m j :
   0 <= j < Q =>
-  Pr[SplitForker(F).run2(i, j) @ &m : res.`1 = j /\ res.`2 = j] =
-  Pr[InitRewinder(F).main((i, j)) @ &m : res.`1.`2.`1.`1 = j /\ res.`2.`2.`1.`1 = j].
+  Pr[SplitForker(I, F).run2(j) @ &m : res.`1 = j /\ res.`2 = j] =
+  Pr[InitRewinder(I, F).main(j) @ &m : res.`1.`2.`1.`1 = j /\ res.`2.`2.`1.`1 = j].
 proof.
 move => j_range.
 byequiv (init_rew_split_equiv j j_range) => /#.
 qed.
 
-local lemma pr_fork_specific &m i j :
+local lemma pr_fork_specific &m j :
   0 <= j < Q =>
-  Pr[Forker(F).run(i) @ &m : Forker.j1 = j /\ Forker.j2 = j] >=
-  Pr[Runner(F, FRO).run(i) @ &m : res.`1 = j] ^ 2.
+  Pr[IForker(I, F).run() @ &m : IForker.j1 = j /\ IForker.j2 = j] >=
+  Pr[IRunner(I, F, FRO).run() @ &m : res.`1 = j] ^ 2.
 proof.
 move => j_range.
 rewrite pr_run1_eq //.
-move : (pr_run2_ineq &m i j).
+move : (pr_run2_ineq &m j).
 apply ler_trans.
 rewrite pr_wrapper_run //.
 rewrite pr_wrapper_main //.
@@ -984,21 +1056,21 @@ qed.
  * Put all the pieces together.
  *)
 
-lemma pr_fork_success &m i :
-  let pr_runner_succ = Pr[Runner(F, FRO).run(i) @ &m : success res.`1] in
-  let pr_fork_succ   = Pr[Forker(F).run(i) @ &m : success res.`1] in
+lemma pr_fork_success &m :
+  let pr_runner_succ = Pr[IRunner(I, F, FRO).run() @ &m : success res.`1] in
+  let pr_fork_succ   = Pr[IForker(I, F).run() @ &m : success res.`1] in
   pr_fork_succ >= pr_runner_succ ^ 2 / Q%r - pr_runner_succ * pr_collision.
 proof.
 simplify.
 rewrite fork_pr.
-move : (pr_split i &m).
+move : (pr_split &m).
 apply ler_trans.
 apply ler_sub; first last.
 + apply pr_succ_resp_eq.
 rewrite pr_split_sum.
 rewrite pr_succ_sum.
-have : bigi predT (fun (j : int) => Pr[Runner(F, FRO).run(i) @ &m : res.`1 = j] ^ 2) 0 Q <=
-  bigi predT (fun (j : int) => Pr[Forker(F).run(i) @ &m : Forker.j1 = j /\ Forker.j2 = j]) 0 Q.
+have : bigi predT (fun (j : int) => Pr[IRunner(I, F, FRO).run() @ &m : res.`1 = j] ^ 2) 0 Q <=
+  bigi predT (fun (j : int) => Pr[IForker(I, F).run() @ &m : IForker.j1 = j /\ IForker.j2 = j]) 0 Q.
 + apply ler_sum_seq.
   move => j j_range _ /=.
   apply pr_fork_specific.
@@ -1013,38 +1085,40 @@ section PROPERTY_TRANSFER.
 
 (* In this section, we show that if the result of running F with FRO
  * satisfies some property P_out, then this property also holds for
- * the two results produced by Forker (provided that it succeeds). *)
+ * the two results produced by IForker (provided that it succeeds). *)
 
-declare pred P_in : glob F * in_t.
-declare pred P_out : out_t * (log_t list).
+declare pred P_in : glob I * glob F.
+declare pred P_out : glob I * out_t * (log_t list).
 
 declare axiom run_prop :
-  hoare[Runner(F, Log(FRO)).run : P_in (glob F, i) /\ Log.log = [] ==> P_out (res, Log.log)].
+  hoare[
+    IRunner(I, F, Log(FRO)).run :
+    P_in (glob I, glob F) /\ Log.log = [] ==>
+    P_out (glob I, res, Log.log)
+  ].
 
 local hoare fst_run_prop :
-  Forker(F).fst : P_in (glob F, i) ==> P_out (res.`1, res.`2).
+  IForker(I, F).fst : P_in (glob I, glob F) ==> P_out (glob I, res.`1, res.`2).
 proof.
-conseq (fst_run_log_equiv []) (_ : P_in (glob F, i) /\ Log.log = [] ==> P_out (res, Log.log)) => //.
-+ smt().
-apply run_prop.
+conseq (fst_run_log_equiv []) run_prop => /#.
 qed.
 
 local lemma snd_run_prop_split :
-  (forall j, 0 <= j < Q => hoare[Forker(F).run : P_in (glob F, i) ==> res.`1 = j => P_out ((res.`1, res.`3), Forker.log2)]) =>
-  hoare[Forker(F).run : P_in (glob F, i) ==> success res.`1 => P_out ((res.`1, res.`3), Forker.log2)].
+  (forall j, 0 <= j < Q => hoare[IForker(I, F).run : P_in (glob I, glob F) ==> res.`1 = j => P_out (glob I, (res.`1, res.`3), IForker.log2)]) =>
+  hoare[IForker(I, F).run : P_in (glob I, glob F) ==> success res.`1 => P_out (glob I, (res.`1, res.`3), IForker.log2)].
 proof.
 have snd_forall :
   forall n, 0 <= n =>
-  (forall j, 0 <= j < n => hoare[Forker(F).run : P_in (glob F, i) ==> res.`1 = j => P_out ((res.`1, res.`3), Forker.log2)]) =>
-  hoare[Forker(F).run : P_in (glob F, i) ==> 0 <= res.`1 < n => P_out ((res.`1, res.`3), Forker.log2)].
+  (forall j, 0 <= j < n => hoare[IForker(I, F).run : P_in (glob I, glob F) ==> res.`1 = j => P_out (glob I, (res.`1, res.`3), IForker.log2)]) =>
+  hoare[IForker(I, F).run : P_in (glob I, glob F) ==> 0 <= res.`1 < n => P_out (glob I, (res.`1, res.`3), IForker.log2)].
 + apply ge0ind => /=.
   + smt().
   + move => _.
     by conseq (_ : _ ==> true); 1: smt().
   move => n n_ge0 ind _ ass.
   conseq
-    (_ : _ ==> 0 <= res.`1 < n => P_out ((res.`1, res.`3), Forker.log2))
-    (_ : _ ==>      res.`1 = n => P_out ((res.`1, res.`3), Forker.log2)) => //.
+    (_ : _ ==> 0 <= res.`1 < n => P_out (glob I, (res.`1, res.`3), IForker.log2))
+    (_ : _ ==>      res.`1 = n => P_out (glob I, (res.`1, res.`3), IForker.log2)) => //.
   + smt().
   + apply (ass n).
     smt().
@@ -1055,7 +1129,7 @@ apply snd_forall.
 smt(Q_pos).
 qed.
 
-local lemma split_snd_ll : islossless SplitForker(F).snd.
+local lemma split_snd_ll : islossless SplitForker(I, F).snd.
 proof.
 islossless.
 + apply F_finish_ll.
@@ -1079,16 +1153,16 @@ qed.
 local lemma run1_run2_equiv j0 :
   0 <= j0 < Q =>
   equiv[
-    SplitForker(F).run1 ~ SplitForker(F).run2 :
-    ={glob F, arg} /\ arg{1}.`2 = j0 ==>
-    res{1}.`1 = res{2}.`1 /\ (res{1}.`1 = j0 => ={glob F, res})
+    SplitForker(I, F).run1 ~ SplitForker(I, F).run2 :
+    ={glob I, glob F, arg} /\ arg{1} = j0 ==>
+    res{1}.`1 = res{2}.`1 /\ (res{1}.`1 = j0 => ={glob I, glob F, res})
   ].
 proof.
 move => j0_range.
 proc => /=.
-seq 3 3 : (={glob F, j, j1, a1, o1, log1, sts1} /\ j{1} = j0).
+seq 3 3 : (={glob I, glob F, j, j1, a1, o1, log1, sts1} /\ j{1} = j0).
 + wp.
-  call (_ : ={glob F}).
+  call (_ : ={glob I, glob F}).
   + sim; auto.
   auto.
 case (j1{1} = j{1}).
@@ -1101,12 +1175,12 @@ auto => />.
 qed.
 
 local equiv init_rew_snd_equiv :
-  InitRewinder(F).main ~ InitRewinder(F).main_run :
-  ={glob F, arg} ==> res{1}.`2 = res{2}.
+  InitRewinder(I, F).main ~ InitRewinder(I, F).main_run :
+  ={glob I, glob F, arg} ==> ={glob I} /\ res{1}.`2 = res{2}.
 proof.
 proc => /=.
 call (_ : ={glob F}); 1: sim.
-inline InitRewinder(F).A.getState InitRewinder(F).A.setState.
+inline InitRewinder(I, F).A.getState InitRewinder(I, F).A.setState.
 elim F_rewindable => enc_glob [_ [get_st_pr [set_st_pr set_st_ll]]].
 have set_st_ph : forall gF,
   phoare[F.setState : arg = enc_glob gF ==> (glob F) = gF] = 1%r.
@@ -1114,7 +1188,7 @@ have set_st_ph : forall gF,
   bypr => &m.
   by apply set_st_pr.
 ecall {1} (set_st_ph (glob F){2}).
-inline InitRewinder(F).A.run.
+inline InitRewinder(I, F).A.run.
 wp.
 call {1} split_snd_ll.
 wp.
@@ -1125,43 +1199,43 @@ have get_st_ph : forall gF,
   move => <-.
   by apply get_st_pr.
 ecall {1} (get_st_ph (glob F){2}).
-conseq (_ : _ ==> ={glob F, r0}) => //.
+conseq (_ : _ ==> ={glob I, glob F, r0}) => //.
 sim.
 qed.
 
 local lemma snd_run_prop_single j0 :
   0 <= j0 < Q =>
-  hoare[Forker(F).run : P_in (glob F, arg) ==> res.`1 = j0 => P_out ((res.`1, res.`3), Forker.log2)].
+  hoare[IForker(I, F).run : P_in (glob I, glob F) ==> res.`1 = j0 => P_out (glob I, (res.`1, res.`3), IForker.log2)].
 proof.
 move => j0_range.
 conseq
-  (_ : P_in (glob F, arg) ==> Forker.j1 = j0 => P_out ((Forker.j2, res.`3), Forker.log2))
-  (_ : _ ==> res.`1 = j0 => Forker.j1 = j0 /\ Forker.j2 = j0) => //.
+  (_ : P_in (glob I, glob F) ==> IForker.j1 = j0 => P_out (glob I, (IForker.j2, res.`3), IForker.log2))
+  (_ : _ ==> res.`1 = j0 => IForker.j1 = j0 /\ IForker.j2 = j0) => //.
 + smt().
 + proc.
   seq 9 : true => //.
   auto => /#.
 conseq (run_run1_equiv j0 j0_range)
-  (_ : P_in (glob F, arg.`1) /\ arg.`2 = j0 ==> res.`1 = j0 => P_out ((res.`2, res.`4), res.`6)).
+  (_ : P_in (glob I, glob F) /\ arg = j0 ==> res.`1 = j0 => P_out (glob I, (res.`2, res.`4), res.`6)).
 + smt().
 + smt().
 conseq (run1_run2_equiv j0 j0_range)
-  (_ : P_in (glob F, arg.`1) /\ arg.`2 = j0 ==> P_out ((res.`2, res.`4), res.`6)).
+  (_ : P_in (glob I, glob F) /\ arg = j0 ==> P_out (glob I, (res.`2, res.`4), res.`6)).
 + smt().
 + smt().
 conseq (init_rew_split_equiv j0 j0_range)
-  (_ : P_in (glob F, arg.`1) /\ arg.`2 = j0 ==> P_out res.`2.`2).
+  (_ : P_in (glob I, glob F) /\ arg = j0 ==> P_out (glob I, res.`2.`2.`1, res.`2.`2.`2)).
 + smt().
 + smt().
-conseq init_rew_snd_equiv (_ : P_in (glob F, arg.`1) /\ arg.`2 = j0 ==> P_out res.`2).
+conseq init_rew_snd_equiv (_ : P_in (glob I, glob F) /\ arg = j0 ==> P_out (glob I, res.`2.`1, res.`2.`2)).
 + smt().
 + smt().
 have main_run_equiv_rev :
   forall log0,
   equiv[
-    InitRewinder(F).main_run ~ Runner(F, Log(FRO)).run :
-    ={glob F} /\ arg{1} = (arg{2}, j0) /\ Log.log{2} = log0 ==>
-    res{1}.`2.`1 = res{2} /\ log0 ++ res{1}.`2.`2 = Log.log{2}
+    InitRewinder(I, F).main_run ~ IRunner(I, F, Log(FRO)).run :
+    ={glob I, glob F} /\ arg{1} = j0 /\ Log.log{2} = log0 ==>
+    ={glob I} /\ res{1}.`2.`1 = res{2} /\ log0 ++ res{1}.`2.`2 = Log.log{2}
   ].
 + by move => log0; symmetry; conseq (main_run_equiv j0 log0 j0_range).
 conseq (main_run_equiv_rev []) run_prop.
@@ -1170,17 +1244,17 @@ conseq (main_run_equiv_rev []) run_prop.
 qed.
 
 hoare property_transfer :
-  Forker(F).run :
-  P_in (glob F, i) ==>
+  IForker(I, F).run :
+  P_in (glob I, glob F) ==>
   let (j, a1, a2) = res in success j =>
-    P_out ((j, a1), Forker.log1) /\ P_out ((j, a2), Forker.log2).
+    P_out (glob I, (j, a1), IForker.log1) /\ P_out (glob I, (j, a2), IForker.log2).
 proof.
 conseq
-  (_ : _ ==> success res.`1 => P_out ((res.`1, res.`3), Forker.log2))
-  (_ : _ ==> success res.`1 => P_out ((res.`1, res.`2), Forker.log1)) => //.
+  (_ : _ ==> success res.`1 => P_out (glob I, (res.`1, res.`3), IForker.log2))
+  (_ : _ ==> success res.`1 => P_out (glob I, (res.`1, res.`2), IForker.log1)) => //.
 + smt().
 + proc => /=.
-  seq 9 : (P_out ((Forker.j1, a1), Forker.log1)); first last.
+  seq 9 : (P_out (glob I, (IForker.j1, a1), IForker.log1)); first last.
   + auto => /#.
   wp; call (_ : true) => //; call (_ : true); wp.
   call fst_run_prop.
@@ -1192,30 +1266,30 @@ qed.
 end section PROPERTY_TRANSFER.
 
 hoare success_log_props :
-  Forker(F).run : true ==>
+  IForker(I, F).run : true ==>
   let j = res.`1 in
-  let (q1, r1) = nth witness Forker.log1 j in
-  let (q2, r2) = nth witness Forker.log2 j in
+  let (q1, r1) = nth witness IForker.log1 j in
+  let (q2, r2) = nth witness IForker.log2 j in
     success j =>
-      size Forker.log1 = Q /\ size Forker.log2 = Q /\
-      take j Forker.log1 = take j Forker.log2 /\
+      size IForker.log1 = Q /\ size IForker.log2 = Q /\
+      take j IForker.log1 = take j IForker.log2 /\
       q1 = q2 /\ r1 <> r2.
 proof.
 conseq
   (_ : _ ==>
-    let j = res.`1 in success j => size Forker.log1 = Q /\ size Forker.log2 = Q)
+    let j = res.`1 in success j => size IForker.log1 = Q /\ size IForker.log2 = Q)
   (_ : _ ==>
     let j = res.`1 in
-    let (q1, r1) = nth witness Forker.log1 j in
-    let (q2, r2) = nth witness Forker.log2 j in
-      success j => take j Forker.log1 = take j Forker.log2 /\ q1 = q2 /\ r1 <> r2);
+    let (q1, r1) = nth witness IForker.log1 j in
+    let (q2, r2) = nth witness IForker.log2 j in
+      success j => take j IForker.log1 = take j IForker.log2 /\ q1 = q2 /\ r1 <> r2);
 1: smt(); first last.
-+ conseq (property_transfer predT (fun (r : out_t * log_t list) => size r.`2 = Q) _); 1: smt().
-  conseq (run_log_size F FRO).
++ conseq (property_transfer predT (fun (r : glob I * out_t * log_t list) => size r.`3 = Q) _); 1: smt().
+  conseq (irun_log_size I F FRO).
 proc.
 wp.
 have snd_head : forall q0, hoare[
-  Forker(F).snd : q = q0 ==> (head witness res.`2).`1 = q0
+  IForker(I, F).snd : q = q0 ==> (head witness res.`2).`1 = q0
 ].
 + move => q0.
   proc; inline Log.
@@ -1251,50 +1325,54 @@ section CONVENIENCE.
 (* Here we just combine all results we have into a (hopefully)
  * more usable package. *)
 
-declare pred P_in : glob F * in_t.
-declare pred P_out : out_t * (log_t list).
+declare pred P_in : glob I * glob F.
+declare pred P_out : glob I * out_t * (log_t list).
 
 declare axiom success_impl :
-  hoare[Runner(F, Log(FRO)).run : P_in (glob F, i) /\ Log.log = [] ==> success res.`1 => P_out (res, Log.log)].
+  hoare[
+    IRunner(I, F, Log(FRO)).run :
+    P_in (glob I, glob F) /\ Log.log = [] ==>
+    success res.`1 => P_out (glob I, res, Log.log)
+  ].
 
 declare op pr_success : real.
 
 declare axiom success_eq :
-  phoare[Runner(F, FRO).run : P_in (glob F, i) ==> success res.`1] = pr_success.
+  phoare[IRunner(I, F, FRO).run : P_in (glob I, glob F) ==> success res.`1] = pr_success.
 
 lemma forking_lemma :
   phoare[
-    Forker(F).run :
-    P_in (glob F, arg) ==>
+    IForker(I, F).run :
+    P_in (glob I, glob F) ==>
     let (j, a1, a2) = res in
-    let log1 = Forker.log1 in
-    let log2 = Forker.log2 in
+    let log1 = IForker.log1 in
+    let log2 = IForker.log2 in
     let (q1, r1) = nth witness log1 j in
     let (q2, r2) = nth witness log2 j in
     success j /\
     size log1 = Q /\ size log2 = Q /\
     take j log1 = take j log2 /\ q1 = q2 /\ r1 <> r2 /\
-    P_out ((j, a1), log1) /\ P_out ((j, a2), log2)
+    P_out (glob I, (j, a1), log1) /\ P_out (glob I, (j, a2), log2)
   ] >= (pr_success ^ 2 / Q%r - pr_success * pr_collision).
 proof.
 conseq (_ : _ ==> success res.`1) (_ : _ ==>
   success res.`1 =>
     let (j, a1, a2) = res in
-    let log1 = Forker.log1 in
-    let log2 = Forker.log2 in
+    let log1 = IForker.log1 in
+    let log2 = IForker.log2 in
     let (q1, r1) = nth witness log1 j in
     let (q2, r2) = nth witness log2 j in
     size log1 = Q /\ size log2 = Q /\
     take j log1 = take j log2 /\ q1 = q2 /\ r1 <> r2 /\
-    P_out ((j, a1), log1) /\ P_out ((j, a2), log2)).
+    P_out (glob I, (j, a1), log1) /\ P_out (glob I, (j, a2), log2)).
 + trivial.
 + smt().
-+ pose P_out' := fun (ol : out_t * (log_t list)) => success ol.`1.`1 => P_out ol.
++ pose P_out' := fun (ol : glob I * out_t * (log_t list)) => success ol.`2.`1 => P_out ol.
   conseq success_log_props (property_transfer P_in P_out' success_impl) => /#.
 bypr => &m P_in_arg /=.
-have -> : pr_success = Pr[Runner(F, FRO).run(arg{m}) @ &m : success res.`1].
-+ by byphoare (_ : glob F = (glob F){m} /\ arg = arg{m} ==> _) => //; conseq success_eq.
-apply (pr_fork_success &m arg{m}).
+have -> : pr_success = Pr[IRunner(I, F, FRO).run() @ &m : success res.`1].
++ by byphoare (_ : (glob I, glob F) = (glob I, glob F){m} /\ arg = arg{m} ==> _) => //; conseq success_eq.
+apply (pr_fork_success &m).
 qed.
 
 end section CONVENIENCE.
